Got a top level repl theorem in the basis env
There is 1 cheat in replCorrect dealing with bytecode termination. There
are 2 cheats in initialProgram, 1 dealing with bytecode termination, and
1 because we can no longer CBV_CONV the primitive program's bytecode
program, but we need that concretely to establish the primitive
program's invariant.

initial/proofs/initialProgramScript.sml
@@ -75,22 +75,44 @@ add_to_sem_env se prog =
 val compile_thm =
   SIMP_RULE (srw_ss()++boolSimps.DNF_ss) [AND_IMP_INTRO, evaluate_whole_prog_def] compilerProofTheory.compile_initial_prog_thm;
 
+val empty_bc_state_def = Define `
+empty_bc_state = <| 
+      stack := [];
+      code := [];
+      pc := 0;
+      refs := FEMPTY;
+      globals := [];
+      handler := 0;
+      output := "";
+      inst_length := real_inst_length;
+      clock := NONE |>`;
+
+val install_code_def = Define `
+  install_code code bs =
+    bs with <| code   := bs.code ++ REVERSE code
+             ; pc     := next_addr bs.inst_length bs.code
+             ; output := ""
+             |>`;
+
 val add_to_env_invariant_lem = Q.prove (
-`!envM envC envE cnt s tids prog cnt' s' envM' envC' envE' tids' mdecls' e e' code bs bs'.
+`!envM envC envE cnt s tids prog cnt' s' envM' envC' envE' tids' mdecls' e e' code code' bs.
   closed_prog prog ∧
   evaluate_whole_prog T (envM,envC,envE) ((cnt,s),tids,set e.inf_mdecls) prog (((cnt',s'),tids',mdecls'),envC',Rval (envM',envE')) ∧
-  invariant <| sem_envM := envM; sem_envC := envC; sem_envE := envE; sem_s := s; sem_tids := tids; sem_mdecls := set e.inf_mdecls |> e bs ∧
-  SOME (e',code) = add_to_env e prog ∧
-  SOME bs' = bc_eval (bs with <| code   := bs.code ++ REVERSE code
-                               ; pc     := next_addr bs.inst_length bs.code |>)
+  SOME bs = bc_eval (install_code code empty_bc_state) ∧
+  invariant <| sem_envM := envM; sem_envC := envC; sem_envE := envE; sem_s := s; sem_tids := tids; sem_mdecls := set e.inf_mdecls |> 
+            e 
+            bs ∧
+  SOME (e',code') = add_to_env e prog
   ⇒
+  ?bs'.
+  SOME bs' = bc_eval (install_code (code'++code) empty_bc_state) ∧
   invariant <| sem_envM := envM' ++ envM;
                sem_envC := merge_envC envC' envC;
                sem_envE := envE' ++ envE;
                sem_s := s';
                sem_tids := tids';
                sem_mdecls := mdecls' |>
-            e' (bs' with clock := NONE)`,
+            e' bs'`,
  rw [add_to_env_def, LET_THM] >>
  every_case_tac >>
  fs [] >>
@@ -121,7 +143,7 @@ val add_to_env_invariant_lem = Q.prove (
  rw [] >>
  fs [union_decls_def, convert_menv_def, typeSysPropsTheory.bvl2_append, convert_env2_def] >>
  rw [] >>
- qabbrev_tac `bs1 = bs with <| clock := SOME cnt; code := bs.code++REVERSE code; pc := next_addr bs.inst_length bs.code |>` >>
+ qabbrev_tac `bs1 = bs with <| clock := SOME cnt; code := bs.code++REVERSE code'; pc := next_addr bs.inst_length bs.code |>` >>
  qabbrev_tac `bc0 = bs.code` >>
  `env_rs (envM,envC,envE) ((cnt,s),tids,set e.inf_mdecls) (genv,gtagenv,rd) e.comp_rs (bs1 with code := bc0)`
              by (UNABBREV_ALL_TAC >>
@@ -131,7 +153,7 @@ val add_to_env_invariant_lem = Q.prove (
                  match_mp_tac compilerProofTheory.env_rs_change_clock >>
                  first_assum(match_exists_tac o concl) >>
                  simp[bc_state_component_equality]) >>
- `bs1.code = bc0 ++ REVERSE code`
+ `bs1.code = bc0 ++ REVERSE code'`
              by (UNABBREV_ALL_TAC >>
                  rw [bc_state_fn_updates]) >>
  `IS_SOME bs1.clock`
@@ -146,50 +168,59 @@ val add_to_env_invariant_lem = Q.prove (
  fs [] >>
  pop_assum(mp_tac o MATCH_MP (REWRITE_RULE[GSYM AND_IMP_INTRO] compilerProofTheory.env_rs_change_clock)) >>
  simp[] >> disch_then(qspecl_then[`0`,`NONE`]mp_tac) >> simp[] >> strip_tac >>
- `bc_next^* (bs with <| code := bc0 ++ REVERSE code; pc := next_addr bs.inst_length bc0 |>) bs' ∧
+ (*
+ `bc_next^* (install_code (code' ++ code) empty_bc_state) bs' ∧
   ¬?s3. bc_next bs' s3`
             by metis_tac [bytecodeEvalTheory.bc_eval_SOME_RTC_bc_next] >>
- `bs' = (bs'' with clock := NONE)` by (
+ `bs' = (bs'' with clock := NONE)` by cheat >> (*(
    qmatch_assum_abbrev_tac`bc_next^* bs0 bs'` >>
    qspecl_then[`bs1`,`bs''`]mp_tac bytecodeClockTheory.RTC_bc_next_can_be_unclocked >>
    discharge_hyps >- simp[] >> strip_tac >>
    `bs1 with clock := NONE = bs0` by (
-     simp[Abbr`bs0`,Abbr`bs1`,bc_state_component_equality] ) >>
+     simp[Abbr`bc0`,Abbr`bs0`,Abbr`bs1`,bc_state_component_equality, install_code_def, empty_bc_state_def]) >>
    fs[] >>
    qspecl_then[`bs0`,`bs'' with clock := NONE`]mp_tac bytecodeEvalTheory.RTC_bc_next_bc_eval >>
    discharge_hyps >- simp[] >>
    discharge_hyps >- (
      simp[bytecodeEvalTheory.bc_eval1_thm,bytecodeEvalTheory.bc_eval1_def,
           bytecodeClockTheory.bc_fetch_with_clock] ) >>
-   rw[] >> fs[] ) >>
+   rw[] >> fs[] ) >> *)
+   *)
  unabbrev_all_tac >>
  fs [] >>
  imp_res_tac RTC_bc_next_preserves >>
  fs [] >>
+ qexists_tac `bs'' with clock := NONE` >>
+ rw []
+ >- cheat >>
  MAP_EVERY qexists_tac [`FST grd''`, `FST (SND grd'')`, `SND (SND grd'')`] >>
  rw []
  >- (imp_res_tac compilerProofTheory.compile_initial_prog_code_labels_ok >>
+     fs [install_code_def] >>
      match_mp_tac bytecodeLabelsTheory.code_labels_ok_append >>
-     simp[])
+     fs [empty_bc_state_def] >>
+     match_mp_tac bytecodeLabelsTheory.code_labels_ok_append >>
+     simp [])
  >- (simp[code_executes_ok_def] >> disj1_tac >>
      metis_tac[bytecodeClockTheory.bc_fetch_with_clock,RTC_REFL]));
 
 val add_to_env_invariant = Q.prove (
-`!ck envM envC envE cnt s tids prog cnt' s' envM' envC' envE' tids' mdecls' e e' code bs bs'.
+`!ck envM envC envE cnt s tids prog cnt' s' envM' envC' envE' tids' mdecls' e e' code code' bs.
   closed_prog prog ∧
   evaluate_whole_prog ck (envM,envC,envE) ((cnt,s),tids,set e.inf_mdecls) prog (((cnt',s'),tids',mdecls'),envC',Rval (envM',envE')) ∧
+  SOME bs = bc_eval (install_code code empty_bc_state) ∧
   invariant <| sem_envM := envM; sem_envC := envC; sem_envE := envE; sem_s := s; sem_tids := tids; sem_mdecls := set e.inf_mdecls |> e bs ∧ 
-  SOME (e',code) = add_to_env e prog ∧
-  SOME bs' = bc_eval (bs with <| code   := bs.code ++ REVERSE code
-                               ; pc     := next_addr bs.inst_length bs.code |>)
+  SOME (e',code') = add_to_env e prog
   ⇒ 
+  ?bs'.
+  SOME bs' = bc_eval (install_code (code'++code) empty_bc_state) ∧
   invariant <| sem_envM := envM' ++ envM;
                sem_envC := merge_envC envC' envC;
                sem_envE := envE' ++ envE;
                sem_s := s';
                sem_tids := tids';
                sem_mdecls := mdecls' |>
-            e' (bs' with clock := NONE)`,
+            e' bs'`,
  rw [] >>
  cases_on `ck`
  >- metis_tac [add_to_env_invariant_lem] >>
@@ -198,7 +229,7 @@ val add_to_env_invariant = Q.prove (
  fs [] >>
  match_mp_tac add_to_env_invariant_lem  >>
  rw [evaluate_whole_prog_def] >>
- MAP_EVERY Q.EXISTS_TAC [`count'`,`s`, `tids`, `prog`, `0`, `e`, `code`, `bs`] >>
+ MAP_EVERY Q.EXISTS_TAC [`count'`,`s`, `tids`, `prog`, `0`, `e`, `bs`] >>
  fs [no_dup_mods_def, no_dup_top_types_def]);
 
 val prim_env_def = Define `
@@ -220,22 +251,15 @@ val prim_sem_env_def = Define `
 prim_sem_env =
 add_to_sem_env <| sem_envM := []; sem_envC := ([],[]); sem_envE := []; sem_s := []; sem_tids := {}; sem_mdecls := {} |> prim_types_program`;
 
-val empty_bc_state_def = Define `
-empty_bc_state = <| 
-      stack := [];
-      code := [];
-      pc := 0;
-      refs := FEMPTY;
-      globals := [];
-      handler := 0;
-      output := "";
-      inst_length := real_inst_length;
-      clock := NONE |>`;
-
 val prim_bs_def = Define `
-prim_bs = bc_eval (empty_bc_state 
-                   with <| code   := empty_bc_state.code ++ REVERSE (SND (THE prim_env))
-                         ; pc     := next_addr empty_bc_state.inst_length empty_bc_state.code |>)`
+prim_bs = bc_eval (install_code (SND (THE prim_env)) empty_bc_state)`;
+
+(* TODO: This is too slow (diverging?), but we need the value
+val prim_bs_eq = 
+  ``prim_bs``
+     |> SIMP_CONV (srw_ss()) [install_code_def, prim_bs_def, prim_env_def, empty_bc_state_def]
+     |> CONV_RULE (computeLib.CBV_CONV the_bytecode_compset)
+     *)
 
 val the_compiler_compset = the_compiler_compset false
 
@@ -249,12 +273,6 @@ val prim_sem_env_eq = save_thm ("prim_sem_env_eq",
   ``prim_sem_env``
   |> SIMP_CONV(srw_ss())[prim_sem_env_def,add_to_sem_env_def,prim_types_program_def]
   |> CONV_RULE(computeLib.CBV_CONV the_interp_compset));
-
-  (*
-val prim_bs_eq = save_thm ("prim_bs_eq",
-  ``prim_bs``
-  |> SIMP_CONV(srw_ss())[prim_bs_def, empty_bc_state_def, prim_env_eq]
-  |> CONV_RULE(computeLib.CBV_CONV the_bytecode_compset));
 
 val to_ctMap_list_def = Define `
 to_ctMap_list tenvC =
@@ -272,9 +290,14 @@ val prim_env_inv = Q.store_thm ("prim_env_inv",
 `?se e code bs.
   prim_env = SOME (e,code) ∧
   prim_sem_env = SOME se ∧
-  prim_bs = SOME bs ∧
+  bc_eval (install_code code empty_bc_state) = SOME bs ∧
   invariant se e bs`,
- rw [prim_env_eq, prim_sem_env_eq, invariant_def, prim_bs_eq, GSYM PULL_EXISTS]
+cheat);
+(*
+ rw [prim_bs_eq, prim_env_eq, prim_sem_env_eq, invariant_def, GSYM PULL_EXISTS] >>
+ qexists_tac `bs` >>
+ rw []
+ >- fs [prim_env_eq]
  >- (rw [typeSoundInvariantsTheory.type_sound_invariants_def] >>
      MAP_EVERY qexists_tac [`to_ctMap (FST (THE prim_env)).inf_tenvC`, 
                             `[]`, 
@@ -321,6 +344,7 @@ val prim_env_inv = Q.store_thm ("prim_env_inv",
          metis_tac [weakeningTheory.weak_decls_refl])
      >- rw [prim_env_eq, weak_decls_only_mods_def, convert_decls_def])
  >- rw [infer_sound_invariant_def,check_menv_def,check_cenv_def,check_flat_cenv_def,terminationTheory.check_freevars_def,check_env_def]
+
  >- (simp[compilerProofTheory.env_rs_def,LENGTH_NIL_SYM] >>
      qexists_tac`
       FEMPTY |++ [(("NONE",TypeId (Short "option")), (none_tag, 0));
@@ -332,10 +356,11 @@ val prim_env_inv = Q.store_thm ("prim_env_inv",
               (("Eq",TypeExn (Short "Eq")), (eq_tag,0));
               (("Subscript",TypeExn(Short"Subscript")),(subscript_tag,0))]` >>
      simp[Once RIGHT_EXISTS_AND_THM] >>
-     conj_tac >- EVAL_TAC >>
+     conj_tac >- cheat >>
      simp[PULL_EXISTS] >>
      CONV_TAC SWAP_EXISTS_CONV >> qexists_tac`[]` >> simp[RIGHT_EXISTS_AND_THM] >>
      simp[RIGHT_EXISTS_AND_THM,GSYM CONJ_ASSOC] >>
+     conj_tac >- cheat >>
      conj_tac >- (EVAL_TAC >> simp[s_to_i1_cases] >> simp[Once v_to_i1_cases] >> simp[Once v_to_i1_cases]) >>
      CONV_TAC SWAP_EXISTS_CONV >> qexists_tac`[]` >>
      CONV_TAC SWAP_EXISTS_CONV >> qexists_tac`[]` >>
@@ -380,8 +405,8 @@ val prim_env_inv = Q.store_thm ("prim_env_inv",
      simp[] >>
      CONV_TAC (computeLib.CBV_CONV the_bytecode_compset) ) >>
    metis_tac[bytecodeEvalTheory.bc_eval_SOME_RTC_bc_next]))
+   *)
 
- (*
 val basis_env_def = Define `
 basis_env =
 add_to_env (FST (THE prim_env)) basis_program`;
@@ -389,11 +414,6 @@ add_to_env (FST (THE prim_env)) basis_program`;
 val basis_sem_env_def = Define `
 basis_sem_env =
 add_to_sem_env (THE prim_sem_env) basis_program`;
-
-val basis_bs_def = Define `
-basis_bs = bc_eval (THE prim_bs 
-                    with <| code   := (THE prim_bs).code ++ REVERSE (SND (THE basis_env))
-                          ; pc     := next_addr (THE prim_bs).inst_length (THE prim_bs).code |>)`
 
 val basis_env_eq = save_thm ("basis_env_eq",
   ``basis_env``
@@ -409,27 +429,16 @@ val basis_sem_env_eq = save_thm ("basis_sem_env_eq",
   |> CONV_RULE(computeLib.CBV_CONV the_interp_compset));
   *)
 
-(* This also takes too long, probably due to linear lookup of instruction fetching *)
-val basis_bs_eq = save_thm ("basis_bs_eq",
-  ``basis_bs``
-  |> SIMP_CONV std_ss [prim_bs_eq, basis_bs_def, basis_env_eq]
-  |> CONV_RULE(computeLib.CBV_CONV the_bytecode_compset)
-
 val basis_env_inv = Q.store_thm ("basis_env_inv",
 `?se e code bs.
   basis_env = SOME (e,code) ∧
   basis_sem_env = SOME se ∧
-  basis_bs = SOME bs ∧
+  SOME bs = bc_eval (install_code (code ++ SND (THE prim_env)) empty_bc_state) ∧
   invariant se e bs`,
- rw [basis_env_def, basis_sem_env_def] >>
+ rw [basis_env_def] >>
  strip_assume_tac prim_env_inv >>
- `?e'. add_to_env e basis_program = SOME e'` by (
-   fs[prim_env_eq] >> rw[] >>
-   simp[add_to_env_def] >>
-   rpt BasicProvers.CASE_TAC >- simp[UNCURRY] >>
-   qsuff_tac`F`>-rw[]>>pop_assum mp_tac>>
-   simp[basis_program_def,mk_binop_def,mk_unop_def] >>
-   CONV_TAC(computeLib.CBV_CONV the_inference_compset)) >>
+ `?e' code. basis_env = SOME (e',code)` by rw [basis_env_eq] >>
+ fs [basis_env_def] >>
  `?se'. add_to_sem_env se basis_program = SOME se'` by (
    fs[prim_sem_env_eq] >> rw[] >>
    simp[add_to_sem_env_def] >>
@@ -463,7 +472,7 @@ val basis_env_inv = Q.store_thm ("basis_env_inv",
    REWRITE_TAC[mk_unop_def] >> CONV_TAC(computeLib.CBV_CONV the_interp_compset) >>
    rw[]) >>
  rw [] >>
- fs [add_to_sem_env_def] >>
+ fs [add_to_sem_env_def, basis_sem_env_def] >>
  every_case_tac >>
  fs [] >>
  imp_res_tac run_eval_prog_spec >>
@@ -489,8 +498,7 @@ val basis_env_inv = Q.store_thm ("basis_env_inv",
  >- (fs [invariant_def] >>
      metis_tac [])
  >- (fs [invariant_def] >>
-     metis_tac []));
-     *)
+     metis_tac [])
+ >- metis_tac [optionTheory.THE_DEF, FST]);
 
-     *)
 val _ = export_theory();
